ported genLensN to TM.Extractable

plugin-demo/gen-src/demo.v
@@ -1,7 +1,236 @@
 From Template Require Import
      Ast
+     Loader
      TemplateMonad.Extractable.
 
 
 Definition showoff : TM unit :=
   tmMsg "running from an extracted plugin!".
+
+
+Require Import ExtLib.Structures.Functor.
+Require Import ExtLib.Structures.Monad.
+Require Import ExtLib.Structures.MonadState.
+Require Import ExtLib.Structures.MonadExc.
+
+Set Primitive Projections.
+
+Record Lens (a b c d : Type) : Type :=
+{ view : a -> c
+; over : (c -> d) -> a -> b
+}.
+
+Arguments over {_ _ _ _} _ _ _.
+Arguments view {_ _ _ _} _ _.
+
+Definition lens_compose {a b c d e f : Type}
+           (l1 : Lens a b c d) (l2 : Lens c d e f)
+: Lens a b e f :=
+{| view := fun x : a => view l2 (view l1 x)
+ ; over := fun f0 : e -> f => over l1 (over l2 f0) |}.
+
+Infix "∙" := lens_compose (at level 90, left associativity).
+
+Require Import ExtLib.Core.RelDec.
+Definition lensAt {A C} (x : A) {reqd: RelDec (@eq A)}: Lens (A->C) (A->C) C C.
+  constructor.
+  intros f. exact (f x).
+  intros f g x'.
+  exact (if (rel_dec x' x) then (f (g x)) else (g x')).
+Defined.
+
+Section ops.
+  Context {a b c d : Type} (l : Lens a b c d).
+
+  Definition set (new : d) : a -> b :=
+    l.(over) (fun _ => new).
+End ops.
+
+
+Section GuardExc.
+  Context {e} {m} {Monad_m : Monad m} {MonadExc_m : MonadExc e m}.
+
+  Definition guard (err : e) (g : bool) : m unit :=
+    if g then ret tt else raise err.
+End GuardExc.
+
+Import MonadNotation.
+
+Local Open Scope monad_scope.
+
+Definition to_bool {P Q} (x : {P} + {Q}) : bool :=
+  match x with
+  | left _ => true
+  | right _ => false
+  end.
+
+Section stateL.
+  Context {m : Type -> Type} {Monad_m : Monad m} {s} {MS : MonadState s m}.
+
+  Definition modifyL
+             {a} (l : Lens s s a a) (f : a -> a) : m a :=
+    x <- get ;;
+    let res := l.(over) f x in
+    put res ;;
+    ret (l.(view) res).
+
+  Definition putL {a} (l : Lens s s a a) (x : a) : m unit :=
+    modifyL l (fun _ => x) ;; ret tt.
+
+  Definition getL {a} (l : Lens s s a a) : m a :=
+    fmap l.(view) get.
+End stateL.
+
+Lemma view_set : forall {A B} (l : Lens A A B B) x,
+    set l (l.(view) x) x = x.
+Admitted.
+Lemma set_view : forall {A B} (l : Lens A A B B) x r,
+    l.(view) (set l x r) = x.
+Admitted.
+
+
+Set Primitive Projections.
+Set Universe Polymorphism.
+
+Import MonadNotation.
+
+Record Info : Set :=
+{ type : ident
+; ctor : ident
+; fields : list (ident * term)
+}.
+
+Fixpoint countTo (n : nat) : list nat :=
+  match n with
+  | 0 => nil
+  | S m => countTo m ++ (m :: nil)
+  end.
+
+Require Import String.
+Open Scope string_scope.
+Definition prepend (ls : string) (i : ident) : ident :=
+  ls ++ i.
+
+Quote Definition cBuild_Lens := Build_Lens.
+
+Require Import Coq.Lists.List.
+Require Import Coq.Bool.Bool.
+
+Fixpoint boundIn (v : nat) (t : term) : bool.
+refine
+  match t with
+   | tRel n => PeanoNat.Nat.eqb n v
+   | tVar i => _
+   | tMeta n => false
+   | tEvar n l => existsb (boundIn v) l
+   | tSort u => false
+   | tCast t1 c t2 => boundIn v t1 || boundIn v t2
+   | tProd n t1 t2 => boundIn v t1 || boundIn (S v) t2
+   | tLambda n t1 t2 => boundIn v t1 || boundIn (S v) t2
+   | tLetIn n t1 t2 t3 => boundIn v t1 || boundIn v t2 || boundIn (S v) t3
+   | tApp t0 l => boundIn v t0 || existsb (boundIn v) l
+   | tConst k u => false
+   | tInd i u => false
+   | tConstruct i n u => false
+   | tCase p t1 t2 l => _
+   | tProj p t0 => boundIn v t0
+   | tFix m n => _
+   | tCoFix m n => _
+   end.
+Admitted.
+
+(* check to see if Var 0 is referenced in any of the terms *)
+Definition mentions (v : nat) (ls : list (ident * term)) : bool :=
+  false.
+
+
+Definition mkLens (At : term) (fields : list (ident * term)) (i : nat)
+: option (ident * term) :=
+  match At with
+  | tInd ind args =>
+    let ctor := tConstruct ind 0 args in
+    match nth_error fields i with
+    | None => None
+    | Some (name, Bt) =>
+      if mentions 1 (skipn (S i) fields)
+      then None
+      else
+        let p (x : nat) : projection := (ind, 0, x) in
+        let get_body := tProj (p i) (tRel 0) in
+        let f x :=
+            let this := tProj (p x) (tRel 0) in
+            if PeanoNat.Nat.eqb x i
+            then tApp (tRel 1) (this :: nil)
+            else this
+        in
+        let update_body :=
+            tApp ctor (map f (countTo (List.length fields)))
+        in
+        Some ( prepend "_" name
+             , tApp cBuild_Lens
+                    (At :: At :: Bt :: Bt ::
+                        tLambda nAnon At get_body ::
+                        tLambda nAnon (tProd nAnon Bt Bt) (tLambda nAnon At update_body) ::
+                        nil))
+    end
+  | _ => None
+  end.
+
+Definition getFields (mi : mutual_inductive_body)
+: option Info :=
+  match mi.(ind_bodies) with
+  | oib :: nil =>
+    match oib.(ind_ctors) with
+    | ctor :: nil =>
+      Some {| type := oib.(ind_name)
+            ; ctor := let '(x,_,_) := ctor in x
+            ; fields := oib.(ind_projs)
+           |}
+    | _ => None
+    end
+  | _ => None
+  end.
+
+Import TemplateMonad.Extractable.
+Require Import Template.BasicAst Template.AstUtils Ast.
+Let TemplateMonad := TM.
+Fixpoint mconcat (ls : list (TemplateMonad unit)) : TemplateMonad unit :=
+  match ls with
+  | nil => tmReturn tt
+  | m :: ms => tmBind m (fun _ => mconcat ms)
+  end.
+
+
+(* baseName should not contain any paths. For example, if the full name
+is A.B.C#D#E#F, baseName should be F. Also, by import ordering,
+ensure that F resolves to  A.B.C#D#E#F. Use Locate to check this.
+
+If the definition of F refers to any other inductive, they should not
+be in the current section(s).
+ *)
+Set Printing All.
+
+Definition genLensN (baseName : String.string) : TM unit :=
+  let name := baseName in
+  let ty :=
+      (Ast.tInd
+   {|
+   BasicAst.inductive_mind := name;
+   BasicAst.inductive_ind := 0 (* TODO: fix for mutual records *) |} List.nil) in
+   tmBind (tmQuoteInductive name) (fun ind =>
+    match getFields ind with
+    | Some info =>
+      let gen i :=
+          match mkLens ty info.(fields) i return TemplateMonad unit with
+          | None => tmFail "failed to build lens"
+          | Some x =>
+            tmBind (tmEval Common.cbv (snd x))
+                   (fun d =>
+                      tmBind
+                        (tmDefinition (fst x) None d)
+                                     (fun _ => tmReturn tt))
+          end
+      in
+      mconcat (map gen (countTo (List.length info.(fields))))
+    | None => tmFail "failed to get info"
+    end).
